disj/DisjDef.v
@@ -1,0 +1,86 @@
+Require Export Tagged LastCommon Disjoint.
+
+Lemma path_nlrcons_edge (* unused *){A : Type} (a b c : A) l f
+      (Hpath : Path f b c (l :>: a))
+  : f a (ne_back l) = true.
+Proof.
+  revert dependent c.
+  induction l; intros; inversion Hpath; subst; cbn in *.
+  - inversion H3. subst b0 b a1. auto.
+  - eauto.
+Qed.
+
+Lemma lc_nil1 {A : Type} `{EqDec A eq} l1 l2 l2' (x : A)
+      (Hlc : last_common' l1 l2 [] l2' x)
+  : Some x = hd_error l1.
+Proof.
+  unfold last_common' in Hlc. destructH.
+  cbn in *.
+  destruct l1;[inversion Hlc0;congruence'|].
+  cbn.
+  f_equal.
+  eapply postfix_hd_eq;eauto.
+Qed.
+
+Lemma lc_cons1 {A : Type} `{EqDec A eq} l1 l2 l1' l2' (x y : A)
+      (Hlc : last_common' l1 l2 (x :: l1') l2' y)
+  : Some x = hd_error l1.
+Proof.
+  unfold last_common' in Hlc. destructH.
+  destruct l1;[inversion Hlc0;congruence'|].
+  cbn.
+  rewrite cons_rcons_assoc in Hlc0.
+  f_equal.
+  eapply postfix_hd_eq;eauto.
+Qed.
+
+Lemma hd_error_ne_front {A : Type} (l : ne_list A)
+  : hd_error l = Some (ne_front l).
+Proof.
+  induction l;cbn;auto.
+Qed.
+
+
+Lemma lc_succ_rt1 {A : Type} `{EqDec A eq} l1 l2 l1' l2' (x y : A)
+      (Hlc : last_common' l1 l2 l1' l2' x)
+      (Hin : y ∈ l1')
+  : y ≻* x | l1.
+Proof.
+  unfold last_common' in Hlc. destructH.
+  eapply splinter_postfix;eauto.
+  eapply splinter_rev. cbn. rewrite rev_rcons. econstructor. econstructor.
+  eapply splinter_single. rewrite <-In_rev. auto.
+Qed.
+
+
+Lemma lc_succ_rt_eq_lc {A : Type} `{EqDec A eq} l1 l2 l1' l2' (x y : A)
+      (Hlc : last_common' l1 l2 l1' l2' x)
+      (Hsucc1 : y ≻* x | l1)
+      (Hsucc2 : y ≻* x | l2)
+      (Hnd1 : NoDup l1)
+      (Hnd2 : NoDup l2)
+  : x = y.
+Proof.
+  unfold last_common' in Hlc. destructH.
+  dependent induction Hsucc1.
+  - clear IHHsucc1.
+    destruct l1';cbn in Hlc0; eapply postfix_hd_eq in Hlc0; eauto.
+    subst a.
+    dependent induction Hsucc2.
+    + destruct l2';cbn in Hlc2; eapply postfix_hd_eq in Hlc2; eauto. subst.
+      exfalso. eapply Hlc1;left; reflexivity.
+    + destruct l2';cbn in Hlc2; eapply postfix_hd_eq in Hlc2 as Heq; eauto.
+      * subst a.
+        eapply splinter_cons in Hsucc2. exfalso. eapply splinter_in in Hsucc2. inversion Hnd2. auto.
+      * eapply IHHsucc2 with (l2':=l2') ; eauto.
+        -- eapply cons_postfix;eauto.
+        -- clear - Hlc1. eapply disjoint_cons2 in Hlc1. firstorder.
+        -- inversion Hnd2. auto.
+  - destruct l1';cbn in Hlc0; eapply postfix_hd_eq in Hlc0 as Heq; eauto.
+    + subst a.
+      eapply splinter_cons in Hsucc1. eapply splinter_in in Hsucc1. inversion Hnd1. subst. contradiction.
+    + eapply IHHsucc1 with (l1':=l1');eauto.
+      * eapply cons_postfix;eauto.
+      * eapply disjoint_cons1 in Hlc1. firstorder.
+      * inversion Hnd1. auto.
+Qed.
