disj/DisjPaths.v
@@ -1,0 +1,242 @@
+Require Export DisjDef MaxPreSuffix.
+
+Section disj.
+  Context `{C : redCFG}.
+  
+  Notation "p '-a>b' q" := (a_edge p q) (at level 55).
+  Notation "p '-a>' q" := (p -a>b q = true) (at level 55).
+  Notation "p '-->b' q" := (edge p q) (at level 55).
+  Notation "p '-->' q" := (p -->b q = true) (at level 55, right associativity).
+  
+(*  Lemma lc_common_element_nin {A : Type}(l1 l2 l1' l2' : list (Lab * Tag)) x y
+        (Hlc : last_common' l1 l2 l1' l2' x)
+        (Hin1 : y ∈ l1)
+        (Hin2 : y ∈ l2)
+    : y ∉ l1' /\ y ∉ l2'.
+  Proof.
+    revert dependent y. revert l1 l2 l1' l2' x Hlc.
+    enough (forall (l1 l2 l1' l2' : list (Lab * Tag)) (x : Lab * Tag),
+               last_common' l1 l2 l1' l2' x -> forall y, y ∈ l1 -> y ∈ l2 -> y ∉ l1').
+    { split;[|eapply last_common'_sym in Hlc];eapply H;eauto. }
+    intros ? ? ? ? ? Hlc y Hin1 Hin2. 
+    unfold last_common' in Hlc. destructH.*)
+
+  Lemma geq_tag_suffix_deq (p q : Lab) l t i j
+        (Hpath : TPath (root,start_tag) (q,j) t)
+        (Hpost : Postfix l t)
+        (HForall : Forall (DecPred (fun xl => |j| <= |snd xl|)) l)
+        (Hel : (p,i) ∈ l)
+    : deq_loop p q.
+  Proof.
+  Admitted.
+
+  Lemma geq_tag_suffix_tag_tl_eq (p q : Lab) l t i j
+        (Hpath : TPath (root,start_tag) (q,j) t)
+        (Hpost : Postfix l t)
+        (HForall : Forall (DecPred (fun xl => |j| <= |snd xl|)) l)
+        (Hel : (p,i) ∈ l)
+    : take_r (| tl j |) i = tl j.
+  Admitted.
+
+  Lemma while'_front_In (A : Type) (e : A -> A -> bool) (P : decPred A) (l : ne_list A) (a b : A)
+        (Hpath : Path e a b l)
+        (HP : P b)
+    : b ∈ while' P l.
+  Proof.
+    destruct Hpath;cbn.
+    - decide (P a);try contradiction. left. auto.
+    - decide (P c);try contradiction. left. auto.
+  Qed.
+  
+  Lemma postfix_ex_cons
+    : forall (A : Type) (l l' : list A) (a : A), Postfix l l' -> exists a' : A, Postfix (l :r: a') (l' :r: a).
+  Proof.
+    intros. eapply postfix_rev_prefix in H. eapply prefix_ex_cons in H. destructH.
+    exists a'. eapply prefix_rev_postfix'. do 2 rewrite rev_rcons. eauto.
+  Qed.
+
+  Lemma eq_loop_same (h h' : Lab)
+        (Heq : eq_loop h h')
+        (Hl : loop_head h)
+        (Hl' : loop_head h')
+    : h = h'.
+  Proof.
+    eapply loop_contains_Antisymmetric.
+    all: unfold eq_loop,deq_loop in *;destructH;eauto using loop_contains_self.
+  Qed.
+  
+  Lemma entry_through_header h p q
+        (Hnin : ~ loop_contains h p)
+        (Hin : loop_contains h q)
+        (Hedge : p --> q)
+    : q = h.
+  Admitted.
+  
+
+  Lemma ex_entry (h p q : Lab) (i j : Tag) t
+        (Hin : innermost_loop h q)
+        (Hnin : ~ loop_contains h p)
+        (Hpath : TPath (root,start_tag) (q,j) t)
+        (Hord : (q,j) ≻* (p,i) | t)
+    : (h,0 :: tl j) ≻* (p,i) | t.
+  Proof.
+    remember (while' (DecPred (fun xl => |j| <= |snd xl|)) t) as t'.
+    assert (Postfix t' t) as Hpost.
+    { eapply while'_postfix;subst t';eauto. }
+    assert (forall xl, xl ∈ t' -> loop_contains h (fst xl)) as Hloop.
+    { intros. destruct xl as [x l]. eapply geq_tag_suffix_deq in H.
+      4: subst t'; eapply while'_Forall.
+      all: cbn;eauto;destruct Hin as [Hin _];eauto.
+    } 
+    inversion Hpost.
+    - subst. eapply splinter_cons in Hord. eapply splinter_in in Hord.
+      specialize (Hloop (p,i)).
+      exploit Hloop.
+      + rewrite H0; auto.
+      + cbn in Hloop. contradiction.
+    - subst l.
+      specialize (rcons_destruct t') as Ht'.
+      destruct Ht'. (* t' is not empty *)
+      { enough ((q,j) ∈ t') as H00 by (rewrite H0 in H00;cbn in H00;contradiction).
+        subst.
+        eapply while'_front_In;eauto. cbn. omega. }
+      destructH.
+      destruct a0 as [h' k].
+      eapply postfix_ex_cons in H1. destructH. erewrite H in H1.
+      assert (h' = h); [|subst h'].
+      { (*
+         * h' is a header
+         * it has an incoming edge from outside of h
+         *)
+        destruct a'.
+        eapply entry_through_header;cycle 1.
+        - destruct Hin as [Hin1 Hin2].
+          enough (deq_loop h' h).
+          { eapply H2. eapply loop_contains_self. eapply loop_contains_loop_head;auto. }
+          eapply deq_loop_trans; eauto.
+          + eapply geq_tag_suffix_deq. 2:eapply Hpost. all: eauto.
+            * rewrite Heqt'. eapply while'_Forall.
+            * rewrite H0. eapply In_rcons. left. auto.
+          + eapply loop_contains_deq_loop;auto.
+        - rewrite H0 in H1. 
+          eapply postfix_path in H1;eauto 1.
+          instantiate (1:=e).
+          admit. (* inversion tactic for paths *)
+        - eapply while'_max in H1;eauto. cbn in H1. contradict H1.
+          admit. (* because depth = length of tag *)
+      }
+      eapply while'_max in H1 as Hmax;[|eauto]. cbn in Hmax.
+      destruct a'. cbn in *. assert (|l| < |j|) as Hmax' by omega.
+      assert (|j| <= |k|) as Hjk.
+      { assert ((h,k) ∈ t') by (rewrite H0;eapply In_rcons;eauto).
+        rewrite Heqt' in H2.
+        eapply while'_forall in H2. cbn in H2. auto. }
+      assert (|l| < |k|) by omega.
+      eapply tag_entry_lt in H2.
+      + destruct j.
+        { exfalso. cbn in Hmax'. omega. }
+        assert (j = tl k).
+        { replace j with (tl (n :: j)) by (cbn;auto). erewrite <-geq_tag_suffix_tag_tl_eq.
+          - rewrite take_r_tl;eauto. cbn. rewrite H2. cbn. cbn in Hmax. rewrite H2 in Hjk. cbn in Hjk. omega.
+          - eauto.
+          - eapply Hpost. 
+          - subst t'. eapply while'_Forall.
+          - rewrite H0. eapply In_rcons. left. eauto.
+        }
+        rewrite H2 in H3. cbn in H3. cbn. subst j k.
+        clear - Hpost Heqt' H0 H Hpath Hord Hin Hnin.
+        eapply postfix_eq in Hpost. destructH.
+        rewrite H,Hpost.
+        rewrite consAppend. 
+        eapply splinter_app; eapply splinter_single.
+        * rewrite H0. eapply In_rcons. auto.
+        * eapply splinter_cons in Hord. eapply splinter_in in Hord.
+          rewrite Hpost in Hord. eapply in_app_or in Hord. destruct Hord;auto.
+          exfalso.
+          rewrite Heqt' in *.
+          eapply geq_tag_suffix_deq in Hpath;cycle 1.
+          -- eapply while'_postfix. symmetry. eauto.
+          -- rewrite Heqt'. eapply while'_Forall.
+          -- rewrite Heqt'. eapply H1.
+          -- eapply Hnin. eapply Hpath. eapply Hin.
+      + rewrite H0 in H1. eapply postfix_path in H1;eauto.
+        rewrite rcons_nl_rcons in H1. simpl_nl' H1.
+        eapply path_nlrcons_edge in H1. simpl_nl' H1. eauto.
+    (*
+     * define t' as the maximal suffix of t with tag dim >= |j|.
+     * then forall x ∈ t', deq_loop x q thus x ∈ h
+     * by definition t = t' or the maximal suffix starts with a loop enter
+       * if t = t', contradiction bc. p ∈ t = t', and p ∈ h
+       * else, ne_back t' = (h,0 :: tl j) and p ∉ t'
+     *)
+  Admitted.
+
+  Variable (t1 t2 : ne_list (Lab * Tag)) (r1 r2 : list (Lab * Tag)) (q1 q2 s : Lab) (j1 j2 k : Tag).
+  Hypotheses (Hpath1 : TPath (root,start_tag) (q1,j1) t1)
+             (Hpath2 : TPath (root,start_tag) (q2,j2) t2)
+             (Hlc : last_common' t1 t2 r1 r2 (s,k))
+             (Hneq : r1 <> r2) (* <-> r1 <> nil \/ r2 <> nil *)
+             (Hloop : eq_loop q1 q2)
+             (Htag : tl j1 = tl j2)
+             (Htagleq : hd 0 j1 <= hd 0 j2).
+
+  Lemma s_deq_q : deq_loop s q1.
+  Proof.
+    intros h Hh.
+    eapply loop_contains_innermost in Hh as Hinner. destructH.
+    eapply eq_loop_innermost in Hinner as Hinner'; eauto.
+    eapply innermost_loop_deq_loop;eauto. 2:eapply Hloop in Hh;auto.
+    eapply path_front in Hpath1 as Hfront1.
+    eapply path_front in Hpath2 as Hfront2.
+    destruct r1, r2.
+    - contradiction.
+    - eapply lc_nil1 in Hlc.
+      rewrite hd_error_ne_front in Hlc. setoid_rewrite Hfront1 in Hlc. inversion Hlc. subst s k.
+      unfold innermost_loop in Hinner. destructH; auto.
+    - eapply last_common'_sym in Hlc. eapply lc_nil1 in Hlc.
+      rewrite hd_error_ne_front in Hlc. setoid_rewrite Hfront2 in Hlc. inversion Hlc. subst s k.
+      unfold innermost_loop in Hinner'. destructH; auto.
+    - decide (loop_contains h' s);[auto|exfalso].
+      assert (p = (q1,j1)); [|subst p].
+      { eapply lc_cons1 in Hlc;rewrite hd_error_ne_front in Hlc;setoid_rewrite Hfront1 in Hlc. inversion Hlc;auto. }
+      assert (p0 = (q2,j2)); [|subst p0].
+      { eapply last_common'_sym in Hlc.
+        eapply lc_cons1 in Hlc;rewrite hd_error_ne_front in Hlc;setoid_rewrite Hfront2 in Hlc. inversion Hlc;auto. }
+      copy Hinner Hinner''.
+      eapply ex_entry in Hinner;eauto.
+      eapply ex_entry in Hinner';eauto.
+      2: eapply last_common'_sym in Hlc.
+      2,3: eapply lc_succ_rt1;eauto.
+      rewrite Htag in Hinner.
+      eapply lc_succ_rt_eq_lc in Hlc;eauto.
+      2,3: eapply tpath_NoDup;eauto.
+      eapply n. inversion Hlc. eapply loop_contains_self. unfold innermost_loop in Hinner''. destructH.
+      eapply loop_contains_loop_head;eauto.
+  Qed.
+    
+  Lemma dep_eq_impl_head_eq (* unused *): depth s = depth q1 -> get_innermost_loop' s = get_innermost_loop' q1.
+  Admitted.
+
+  Lemma r1_in_head_q (* unused *): forall x, x ∈ r1 -> deq_loop (fst x) q1.
+  Admitted.
+  Lemma r2_in_head_q (* unused *): forall x, x ∈ r2 -> deq_loop (fst x) q2.
+  Admitted.
+
+  Lemma no_back_edge (* unused *): forall x, (get_innermost_loop' q1) ≻ x | (map fst r1) :r: s -> False.
+  Admitted.
+
+  Lemma lc_eq_disj
+        (Hdep : depth s = depth q1)
+        (Hjeq : j1 = j2)
+    : Disjoint (map fst r1) (map fst r2).
+  Admitted.
+  
+  Lemma lc_neq_disj
+        (Hdep : depth s = depth q1)
+        (Hjneq : j1 <> j2)
+    : exists r', Prefix ((get_innermost_loop' q1) :: r') (map fst r2)
+            /\ Disjoint (map fst r1) r'.
+  Admitted.
+  (* This section is now similar to the one in the paper *)
+    
+End disj.
