infra/MaxPreSuffix.v
@@ -1,0 +1,92 @@
+Require Export PreSuffix.
+
+Fixpoint while' {A : Type} (P : decPred A) (l : list A) : list A
+  := match l with
+     | nil => nil
+     | a :: l => if decision (P a) then a :: while' P l else nil
+     end.
+
+Definition while {A : Type} (P : decPred A) (l : list A) : list A
+  := rev (while' P (rev l)).
+
+Lemma while'_postfix {A : Type} (P : decPred A) (l l' : list A)
+      (H : while' P l = l')
+  : Postfix l' l.
+Proof.
+  revert dependent l'.
+  induction l; intros; cbn in *; eauto.
+  - subst. constructor.
+  - decide (P a).
+    + destruct l';[congruence|]. inversion H; subst.
+      eapply postfix_cons. eapply IHl. reflexivity.
+    + subst. eapply postfix_nil.
+Qed.
+
+Lemma while_prefix (* unused *){A : Type} (P : decPred A) (l l' : list A)
+      (H : while P l = l')
+  : Prefix l' l.
+Proof.
+  eapply postfix_rev_prefix'.
+  unfold while in H. rewrite <-H.
+  rewrite rev_involutive.
+  eapply while'_postfix;eauto.
+Qed.
+  
+Lemma while'_Forall {A : Type} (P : decPred A) (l : list A)
+  : Forall P (while' P l).
+Proof.
+  induction l;cbn;eauto.
+  decide (P a).
+  - econstructor;eauto.
+  - econstructor.
+Qed.
+  
+Lemma while_Forall {A : Type} (P : decPred A) (l : list A)
+  : Forall P (while P l).
+Proof.
+  unfold while. rewrite Forall_forall. setoid_rewrite <-in_rev. rewrite <-Forall_forall.
+  eapply while'_Forall.
+Qed.
+
+Lemma while'_app {A : Type} (P : decPred A) (l l' : list A)
+      (H : Forall P l)
+  : while' P (l ++ l') = l ++ while' P l'.
+Proof.
+  induction l;cbn;auto.
+  inversion H;subst. exploit IHl.
+  decide (P a);[|contradiction]. rewrite IHl. auto.
+Qed.
+
+Lemma while'_max {A : Type} (P : decPred A) (l l' : list A) a
+      (Hpost : Postfix (l' :r: a) l)
+      (Hw : while' P l = l')
+  : ~ P a.
+Proof.
+  rewrite postfix_eq in Hpost.
+  destructH.
+  rewrite Hpost in Hw.
+  intro N. rewrite while'_app in Hw.
+  - clear - Hw. induction l';cbn in Hw;[congruence|]. eapply IHl'. inversion Hw. rewrite H0 at 1. reflexivity.
+  - rewrite Forall_forall. setoid_rewrite In_rcons. intros. destruct H;subst;auto.
+    eapply Forall_forall in H;eauto. rewrite <-Hw.
+    eapply while'_Forall.
+Qed.
+    
+  
+Lemma while_max (* unused *){A : Type} (P : decPred A) (l l' : list A) a
+      (Hpre : Prefix (a :: l') l)
+      (Hw : while P l = l')
+  : ~ P a.
+Proof.
+  unfold while in Hw.
+  rewrite <-rev_involutive in Hw. eapply rev_injective in Hw.
+  eapply while'_max;eauto.
+  rewrite <-rev_cons. eapply prefix_rev_postfix;eauto.
+Qed.
+
+Lemma while'_forall (A : Type) (P : decPred A) (l : list A) a
+      (Hin : a ∈ while' P l)
+  : P a.
+Proof.
+  eapply Forall_forall;[|eapply Hin]. eapply while'_Forall.
+Qed.
